theories/Clique.v
@@ -1,0 +1,191 @@
+Require Import Coq.Lists.List.
+Require Import Coq.NArith.NArith.
+Require Import Coq.Classes.SetoidTactics.
+Require Import Coq.Classes.Morphisms Coq.Classes.Morphisms_Prop.
+Require Export Coq.Classes.RelationClasses Coq.Relations.Relation_Definitions.
+Require Import Coq.Classes.Equivalence Coq.Program.Basics.
+
+From Hardness Require Import CNFSAT Graph Reduction.
+From Hardness Require Natnat.
+
+Import ListNotations.
+
+Definition sized_clique (g : NGraph.graph) (k : nat) : Prop :=
+  exists (vs : NSet.t),
+    nset_size vs = k /\
+    forall v1 v2,
+      NSet.In v1 vs ->
+      NSet.In v2 vs ->
+      NGraph.rel g v1 v2.
+
+Instance CLIQUE : problem (undirected_graph * N) :=
+  {| ProblemSize := fun '(g, k) => (graph_size (proj1_sig g) + N.to_nat (N.size k))%nat;
+     ProblemYes := fun '(g, k) => sized_clique (proj1_sig g) (N.to_nat k);
+  |}.
+
+Definition unwrap_or {A} : A -> option A -> A :=
+  option_rect (fun _ => A) (fun x => x).
+
+Definition combine_neighbors' (vs1 vs2 : option NSet.t) : NSet.t :=
+  NSet.union (unwrap_or NSet.empty vs1) (unwrap_or NSet.empty vs2).
+
+Definition combine_neighbors (vs1 vs2 : option NSet.t) : option NSet.t :=
+  Some (combine_neighbors' vs1 vs2).
+
+Definition merge_graphs : NGraph.graph -> NGraph.graph -> NGraph.graph :=
+  NMap.map2 combine_neighbors.
+
+Lemma merge_graphs_correct : forall g1 g2 v1 v2,
+    NGraph.rel (merge_graphs g1 g2) v1 v2 <-> (NGraph.rel g1 v1 v2 \/ NGraph.rel g2 v1 v2).
+Proof.
+  unfold merge_graphs, NGraph.rel.
+  intros.
+  split; intro H.
+  - destruct H as [vs [H1 H2]].
+    match goal with
+    | [ _ : ?x = Some _ |- _ ] =>
+      assert (x <> None) as H3 by congruence
+    end.
+    rewrite <-NGraph.M.XMapFacts.in_find_iff in H3.
+    apply NMap.map2_2 in H3.
+    apply NMap.map2_1 with (f := combine_neighbors) in H3.
+    rewrite H1 in H3.
+    cbv [combine_neighbors combine_neighbors'] in H3.
+    inversion H3; clear H3; subst.
+    destruct NMap.find, NMap.find; cbv [unwrap_or option_rect] in *.
+    + apply NSet.union_1 in H2.
+      destruct H2; eauto.
+    + rewrite NGraph.S.union_empty_r in H2.
+      eauto.
+    + rewrite NGraph.S.union_empty_l in H2.
+      eauto.
+    + cbn in H2.
+      rewrite NGraph.S.union_empty_l in H2.
+      apply NGraph.S.XSetFacts.empty_iff in H2.
+      intuition.
+  - destruct H as [[vs [H1 H2]] | [vs [H1 H2]]].
+    + exists (combine_neighbors' (Some vs) (NMap.find v1 g2)).
+      split.
+      * rewrite NMap.map2_1.
+        -- cbv [combine_neighbors].
+           now rewrite H1.
+        -- left.
+           apply NGraph.M.XMapFacts.in_find_iff.
+           congruence.
+      * cbv [combine_neighbors' unwrap_or option_rect].
+        now apply NSet.union_2.
+    + exists (combine_neighbors' (NMap.find v1 g1) (Some vs)).
+      split.
+      * rewrite NMap.map2_1.
+        -- cbv [combine_neighbors].
+           now rewrite H1.
+        -- right.
+           apply NGraph.M.XMapFacts.in_find_iff.
+           congruence.
+      * cbv [combine_neighbors' unwrap_or option_rect].
+        now apply NSet.union_3.
+Qed.
+
+Definition edge (v1 v2 : N * N) : NGraph.graph :=
+  let v1' := Natnat.encodeN v1 in
+  let v2' := Natnat.encodeN v2 in
+  NGraph.add_edge v1' v2' NMap.empty.
+
+Definition undirected_edge (v1 v2 : N * N) : NGraph.graph :=
+  merge_graphs (edge v1 v2) (edge v2 v1).
+
+Definition undirected (g : NGraph.graph) :=
+  forall x y, NGraph.rel g x y -> NGraph.rel g y x.
+
+Import NGraph.R.
+
+Lemma undirected_edge_undirected : forall v1 v2,
+    undirected (undirected_edge v1 v2).
+Proof.
+  intros v1 v2 x y.
+  cbv [undirected_edge edge].
+  intros H.
+  apply merge_graphs_correct in H.
+  apply merge_graphs_correct.
+  destruct H.
+  - apply NGraph.rel_add_edge in H.
+    assert (NGraph.rel NMap.empty U NGraph.id (Natnat.encodeN v1) (Natnat.encodeN v2) == NGraph.id (Natnat.encodeN v1) (Natnat.encodeN v2)) as H0.
+    { now rewrite NGraph.rel_empty, RelUtil.union_empty_l. }
+    apply H0 in H.
+    cbv [NGraph.id] in H; intuition subst.
+    right.
+    apply NGraph.rel_add_edge.
+    assert (NGraph.rel NMap.empty U NGraph.id (Natnat.encodeN v2) (Natnat.encodeN v1) == NGraph.id (Natnat.encodeN v2) (Natnat.encodeN v1)) as H1.
+    { now rewrite NGraph.rel_empty, RelUtil.union_empty_l. }
+    apply H1.
+    cbv [NGraph.id].
+    auto.
+  - apply NGraph.rel_add_edge in H.
+    assert (NGraph.rel NMap.empty U NGraph.id (Natnat.encodeN v2) (Natnat.encodeN v1) == NGraph.id (Natnat.encodeN v2) (Natnat.encodeN v1)) as H0.
+    { now rewrite NGraph.rel_empty, RelUtil.union_empty_l. }
+    apply H0 in H.
+    cbv [NGraph.id] in H; intuition subst.
+    left.
+    apply NGraph.rel_add_edge.
+    assert (NGraph.rel NMap.empty U NGraph.id (Natnat.encodeN v1) (Natnat.encodeN v2) == NGraph.id (Natnat.encodeN v1) (Natnat.encodeN v2)) as H1.
+    { now rewrite NGraph.rel_empty, RelUtil.union_empty_l. }
+    apply H1.
+    cbv [NGraph.id].
+    auto.
+Qed.
+
+Fixpoint edges_for_lit_cl (cl : clause) (cl_name : N) (lit : literal) (v : N * N) : NGraph.graph * N :=
+  match cl with
+  | nil => (NMap.empty, 0)
+  | lit' :: cl' =>
+    let '(edges, l_name) := edges_for_lit_cl cl' cl_name lit v in
+    match lit, lit' with
+    | PosLit v1, NegLit v2
+    | NegLit v1, PosLit v2 =>
+      if N.eq_dec v1 v2
+      then (edges, l_name + 1)
+      else (merge_graphs (undirected_edge (cl_name, l_name) v) edges, l_name + 1)
+    | _, _ =>
+      (merge_graphs (undirected_edge (cl_name, l_name) v) edges, l_name + 1)
+    end
+  end.
+
+Lemma edges_for_lit_cl_correct : forall cl cl_name lit v,
+    let '(g, _) := edges_for_lit_cl cl cl_name lit v in
+    undirected g.
+Proof.
+  induction cl; cbn; intros cl_name lit v.
+  - intros x y H.
+    apply NGraph.rel_empty in H.
+    inversion H.
+  - 
+
+Fixpoint edges_for_lit (f : cnf_formula) (lit : literal) (v : N * N) : NGraph.graph * N :=
+  match f with
+  | nil => (NMap.empty, 0)
+  | cl :: f' =>
+    let '(edges, cl_name) := edges_for_lit f' lit v in
+    let '(lit_edges, _) := edges_for_lit_cl cl cl_name lit v in
+    (merge_graphs edges lit_edges, cl_name + 1)
+  end.
+
+Fixpoint edges_for_clause (f : cnf_formula) (cl : clause) (cl_name : N) : NGraph.graph * N :=
+  match cl with
+  | nil => (NMap.empty, 0)
+  | l :: cl' =>
+    let '(edges, l_name) := edges_for_clause f cl' cl_name in
+    let '(new_edges, _) := edges_for_lit f l (cl_name, l_name) in
+    (merge_graphs edges new_edges, l_name + 1)
+  end.
+
+Fixpoint do_the_thing (f : cnf_formula) : NGraph.graph * N :=
+  match f with
+  | nil => (NMap.empty, 0)
+  | cl :: f' =>
+    let '(g, n) := do_the_thing f' in
+    let '(edges, _) := edges_for_clause f' cl n in
+    (merge_graphs g edges, n + 1)
+  end.
+
+(* Definition cnfsat_to_clique (f : cnf_formula) : NGraph.graph * N := *)
+(*   () *)
