theories/Graph.v
@@ -1,0 +1,23 @@
+From Coq.NArith Require Import NArith.
+From Coq.Structures Require Import OrderedTypeEx.
+From Coq.FSets Require Import FMapList FSetList.
+From CoLoR.Util Require Import FGraph.FGraph.
+
+Require Import Reduction.
+
+Module NSet := FSetList.Make N_as_OT.
+Module NMap := FMapList.Make N_as_OT.
+
+Module NGraph := FGraph.Make NSet NMap.
+
+(* Coercion NGraph.rel : NGraph.graph >-> NGraph.relation_on_X. *)
+
+Definition undirected_graph :=
+  { g : NGraph.graph | forall x y, NGraph.rel g x y -> NGraph.rel g y x }.
+
+Definition nset_size (s : NSet.t) : nat :=
+  NSet.fold (fun _ n => S n) s 0.
+
+(* size of graph = |V| + |E| *)
+Definition graph_size (g : NGraph.graph) : nat :=
+  NMap.fold (fun _ succs n => n + 1 + nset_size succs) g 0.
