theories/Natnat.v
@@ -1,0 +1,93 @@
+Require Import Coq.NArith.NArith.
+
+Require Import Omega.
+
+Fixpoint decode (n : nat) : nat * nat :=
+  match n with
+  | 0 => (0, 0)
+  | S n => let '(a, b) := decode n in
+           match a with
+           | 0 => (S b, 0)
+           | S a => (a, S b)
+           end
+  end.
+
+(* sorta cheating but oh well *)
+Definition decodeN (n : N) : N * N :=
+  let n' := N.to_nat n in
+  let '(a, b) := decode n' in
+  (N.of_nat a, N.of_nat b).
+
+Fixpoint encode_sum (s : nat) : nat -> nat :=
+  fix es_helper b :=
+    match b with
+    | 0 => match s with
+           | 0 => 0
+           | S s => S (encode_sum s s)
+           end
+    | S b => S (es_helper b)
+    end.
+
+Definition encode ab := let '(a, b) := ab in encode_sum (a + b) b.
+
+Definition encodeN ab :=
+  let '(a, b) := ab in
+  N.of_nat (encode (N.to_nat a, N.to_nat b)).
+
+Lemma decode_encode ab : decode (encode ab) = ab.
+Proof.
+  destruct ab as [a b].
+  revert a b.
+  cbv [encode].
+  enough (forall s b, b <= s -> decode (encode_sum s b) = (s - b, b)) as H.
+  { intros.
+    specialize (H (a + b) b).
+    replace (a + b - b) with a in H by omega.
+    apply H; omega.  }
+  intros s.
+  induction s; intros.
+  { replace b with 0 by omega.
+    cbn [encode_sum decode].
+    reflexivity. }
+  { induction b.
+    { cbn [encode_sum decode].
+      rewrite IHs by omega.
+      replace (s - s) with 0 by omega.
+      reflexivity. }
+    { cbn [encode_sum decode] in IHb |- *.
+      rewrite IHb by omega.
+      replace (S s - b) with (S (S s - S b)) by omega.
+      reflexivity. } }
+Qed.
+
+Lemma encode_decode n : encode (decode n) = n.
+Proof.
+  induction n.
+  { reflexivity. }
+  { cbn [decode].
+    cbv [encode] in *.
+    destruct (decode n) as [a b].
+    destruct a.
+    { cbn [plus] in IHn.
+      replace (S b + 0) with (S b) by omega.
+      cbn [encode_sum].
+      omega. }
+    { replace (S a + b) with (S (a + b)) in IHn by omega.
+      replace (a + S b) with (S (a + b)) by omega.
+      cbn [encode_sum] in IHn |- *.
+      omega. } }
+Qed.
+
+Lemma decodeN_encodeN ab : decodeN (encodeN ab) = ab.
+Proof.
+  destruct ab as [a b].
+  cbv [encodeN decodeN].
+  now rewrite Nat2N.id, decode_encode, !N2Nat.id.
+Qed.
+
+Lemma encodeN_decodeN n : encodeN (decodeN n) = n.
+Proof.
+  cbv [encodeN decodeN].
+  destruct decode eqn:Heq.
+  now rewrite !Nat2N.id, <-Heq, encode_decode, N2Nat.id.
+Qed.
